Updated sender streams and bundles. #135

timesyn/CaseStudies/ABP/Sender.thy
@@ -13,10 +13,121 @@ imports SenderAutomaton
 begin
 
 (* ----------------------------------------------------------------------- *)
+  section {* Datatype Conversion *}
+(* ----------------------------------------------------------------------- *)
+
+text {* Inverse of C. *}
+fun invC :: "Sender \<Rightarrow> (nat \<times> bool)" where
+  "invC (C (n,b)) = (n,b)" |
+  "invC n = undefined"
+
+text {* Conversion of a pair (nat,bool) stream into an equivalent receiver stream. *}
+definition natbool2abp :: "(nat \<times> bool) tsyn stream \<rightarrow> Sender tsyn stream" where
+  "natbool2abp \<equiv> tsynMap C"
+
+text {* Conversion of a receiver stream into an equivalent pair (nat,bool) stream. *}
+definition abp2natbool :: "Sender tsyn stream \<rightarrow> (nat \<times> bool) tsyn stream" where
+  "abp2natbool \<equiv> tsynMap invC"
+
+text {* Inverse of B. *}
+fun invB :: "Sender \<Rightarrow> bool" where
+  "invB (B x) = x" |
+  "invB x = undefined"
+
+text {* Conversion of a bool stream into an equivalent receiver stream. *}
+definition bool2abp :: "bool tsyn stream \<rightarrow> Sender tsyn stream" where
+  "bool2abp \<equiv> tsynMap B"
+
+text {* Conversion of a receiver stream into an equivalent bool stream. *}
+definition abp2bool :: "Sender tsyn stream \<rightarrow> bool tsyn stream" where
+  "abp2bool \<equiv> tsynMap invB"
+
+text {* Inverse of C. *}
+fun invA :: "Sender \<Rightarrow> nat" where
+  "invA (A x) = x" |
+  "invA x = undefined"
+
+text {* Conversion of a nat stream into an equivalent receiver stream. *}
+definition nat2abp :: "nat tsyn stream \<rightarrow> Sender tsyn stream" where
+  "nat2abp \<equiv> tsynMap A"
+
+text {* Conversion of a receiver stream into an equivalent nat stream. *}
+definition abp2nat :: "Sender tsyn stream \<rightarrow> nat tsyn stream" where
+  "abp2nat \<equiv> tsynMap invA"
+
+(* ----------------------------------------------------------------------- *)
+  section {* Sender Test Streams and Bundles *}
+(* ----------------------------------------------------------------------- *)
+
+(* Everything works fine for two messages therefore sender changes state *)
+
+definition sndTestInputStreamINoLoss :: "nat tsyn stream" where 
+  "sndTestInputStreamINoLoss \<equiv> <[Msg 1, Msg 2, Msg 1, null]>"
+
+definition sndTestInputStreamAsNoLoss :: "bool tsyn stream" where 
+  "sndTestInputStreamAsNoLoss \<equiv> <[null, Msg True, Msg False, Msg True]>"
+
+lift_definition sndTestInputUbundleNoLoss :: "Sender tsyn SB" is
+  "[\<guillemotright>i \<mapsto> nat2abp\<cdot>sndTestInputStreamINoLoss, \<guillemotright>as \<mapsto> bool2abp\<cdot>sndTestInputStreamAsNoLoss]" 
+  by (simp add: ubWell_def usclOkay_stream_def ctype_tsyn_def sndTestInputStreamINoLoss_def 
+      sndTestInputStreamAsNoLoss_def bool2abp_def nat2abp_def tsynMap_def rangeI)
+
+definition sndTestOutputStreamNoLoss :: "(nat \<times> bool) tsyn stream" where 
+  "sndTestOutputStreamNoLoss \<equiv> <[Msg (1, True), Msg (2, False), Msg (1, True), null]>"
+
+lift_definition sndTestOutputUbundleNoLoss :: "Sender tsyn SB" is
+  "[ds\<guillemotright> \<mapsto> natbool2abp\<cdot>sndTestOutputStreamNoLoss]"
+  by (simp add: ubWell_def usclOkay_stream_def ctype_tsyn_def sndTestOutputStreamNoLoss_def 
+      natbool2abp_def tsynMap_def)
+
+(* One medium loses data or acknowledgement *)
+
+definition sndTestInputStreamIOneLoss :: "nat tsyn stream" where 
+  "sndTestInputStreamIOneLoss \<equiv> <[Msg 1, null, Msg 2, null]>"
+
+definition sndTestInputStreamAsOneLoss :: "bool tsyn stream" where 
+  "sndTestInputStreamAsOneLoss \<equiv> <[null, null, Msg True, Msg False]>"
+
+lift_definition sndTestInputUbundleOneLoss :: "Sender tsyn SB" is
+  "[\<guillemotright>i \<mapsto> tsynMap A\<cdot>sndTestInputStreamIOneLoss,
+    \<guillemotright>as \<mapsto> tsynMap B\<cdot>sndTestInputStreamAsOneLoss]" 
+  by (simp add: ubWell_def usclOkay_stream_def ctype_tsyn_def sndTestInputStreamAsOneLoss_def
+      sndTestInputStreamIOneLoss_def tsynMap_def rangeI)
+
+definition sndTestOutputStreamOneLoss :: "(nat \<times> bool) tsyn stream" where 
+  "sndTestOutputStreamOneLoss \<equiv> <[Msg (1, True), Msg (1, True), Msg (2, False), null]>"
+
+lift_definition sndTestOutputUbundleOneLoss :: "Sender tsyn SB" is
+  "[ds\<guillemotright> \<mapsto> natbool2abp\<cdot>sndTestOutputStreamOneLoss]"
+  by (simp add: ubWell_def usclOkay_stream_def ctype_tsyn_def sndTestOutputStreamOneLoss_def 
+      natbool2abp_def tsynMap_def)
+
+(* Two messages are successive lost by medium therefore there are two messages in the buffer *)
+definition sndTestInputStreamITwoLoss :: "nat tsyn stream" where
+  "sndTestInputStreamITwoLoss \<equiv> <[Msg 1, Msg 2, Msg 3, null, null, null]>"
+
+definition sndTestInputStreamAsTwoLoss :: "bool tsyn stream" where 
+  "sndTestInputStreamAsTwoLoss \<equiv> <[null, null, null, Msg True, Msg False, Msg True]>"
+
+lift_definition sndTestInputUbundleTwoLoss :: "Sender tsyn SB" is
+  "[\<guillemotright>i \<mapsto> nat2abp\<cdot>sndTestInputStreamITwoLoss, \<guillemotright>as \<mapsto> bool2abp\<cdot>sndTestInputStreamAsTwoLoss]" 
+  by (simp add: ubWell_def usclOkay_stream_def ctype_tsyn_def sndTestInputStreamITwoLoss_def
+      sndTestInputStreamAsTwoLoss_def nat2abp_def bool2abp_def tsynMap_def rangeI)
+
+definition sndTestOutputStreamTwoLoss :: "(nat \<times> bool) tsyn stream" where 
+  "sndTestOutputStreamTwoLoss \<equiv> <[Msg (1, True), Msg (1, True), Msg (1, True), Msg (2, False), 
+                                  Msg (3, True), null]>"
+
+lift_definition sndTestOutputUbundleTwoLoss :: "Sender tsyn SB" is
+  "[ds\<guillemotright> \<mapsto> natbool2abp\<cdot>sndTestOutputStreamTwoLoss]"
+  by (simp add: ubWell_def usclOkay_stream_def ctype_tsyn_def sndTestOutputStreamTwoLoss_def 
+      natbool2abp_def tsynMap_def)
+
+(* ----------------------------------------------------------------------- *)
   section {* Automaton Sender Transition Lemmata *}
 (* ----------------------------------------------------------------------- *)
 
-lemma createdsoutput_ubdom: 
+lemma createdsoutput_ubdom:
   "ubDom\<cdot>(createDsOutput a) = {ds\<guillemotright>}"
   by (metis createDsOutput.rep_eq dom_empty dom_fun_upd option.simps(3) ubdom_insert)
 
@@ -110,7 +221,7 @@ lemma sendertransition_ubdom:
       using f_def s_def by force
   qed
 
-lemma sender_automaton_well:
+lemma sendertransition_automaton_well:
   "automaton_well (senderTransition, SenderState.State Sf [], tsynbNull ds\<guillemotright>, {\<guillemotright>i,\<guillemotright>as }, {ds\<guillemotright>})"
   using sendertransition_ubdom by simp
 
